

# Bernoulli Number and Power Sum

Wearry

## Problem Description

Calculate:

$$S_k(n) = \sum_{i=0}^{n-1} i^k$$

## Transform

$$\begin{aligned} S_{m+1}(n) + n^{m+1} &= S_{m+1}(n+1) \\ &= \sum_{k=0}^{n-1} (k+1)^{m+1} \\ &= \sum_{k=0}^{m+1} \binom{m+1}{k} S_k(n) \end{aligned} \tag{1.1}$$

$$\text{Let } \hat{S}_k(n) = \frac{1}{k+1} \sum_{j=0}^k \binom{k+1}{j} B_j n^{k+1-j} \tag{1.2}$$

$$\text{Where } B_i \text{ follow : } \sum_{j=0}^m \binom{m+1}{j} B_j = [m=0] \tag{1.3}$$

## Proof

$$\hat{S}_k(n) = S_k(n)$$

Considering proof below by induction, assume that  $\forall 0 \leq j < m :$   
 $(\hat{S})_j(n) = S_j(n)$ , now to proof  $\hat{S}_m(n) = S_m(n)$ .

Minus  $S_{m+1}(n)$  from both left and right part of equation(1.1):

$$\begin{aligned} n^{m+1} &= \sum_{k=0}^m \binom{m+1}{k} S_k(n) \\ &= \sum_{k=0}^m \binom{m+1}{k} \hat{S}_k(n) + (m+1)\Delta \\ &= \sum_{0 \leq j \leq k \leq m} \binom{m+1}{k} \binom{k+1}{k-j} \frac{B_{k-j} n^{j+1}}{k+1} + (m+1)\Delta \\ &= \sum_{k=0}^m \binom{m+1}{k} \frac{1}{k+1} \sum_{j=0}^k \binom{k+1}{j+1} B_{k-j} n^{j+1} + (m+1)\Delta \\ &= \sum_{k=0}^m \binom{m+1}{k} \sum_{j=0}^k \binom{k}{j} \frac{B_{k-j} n^{j+1}}{j+1} + (m+1)\Delta \\ &= \sum_{j=0}^m \binom{m+1}{j} \frac{1}{j+1} n^{j+1} \sum_{k=j}^m B_{k-j} \binom{m+1-j}{k-j} + (m+1)\Delta \\ &= n^{m+1} + (m+1)\Delta \end{aligned}$$

$$\Delta = 0, \text{Q.E.D.}$$

## Generating Function

Define :

$$G(x) = \sum_{i=1}^{\infty} \frac{1}{i!} x^i, F(x) = \sum_{i=0}^{\infty} \frac{B_i}{i!} x^i$$

Then consider the production of function F and function G:

$$\begin{aligned}
 (F * G)(x) &= \sum_{i=1}^{\infty} \left( \sum_{j=0}^{i-1} B_j \binom{i}{j} \right) x^i \\
 &= \sum_{i=1}^{\infty} [i - 1 = 0] x^i \\
 &= x \\
 F(x) &= \frac{x}{e^x - 1}
 \end{aligned}$$